theories/rust_typing/base.v
@@ -63,29 +63,6 @@ Class LayoutSizeLe (ly1 ly2 : layout) := layout_size_le_proof : ly_size ly1 ≤ 
 Global Instance layout_size_le_refl ly : LayoutSizeLe ly ly.
 Proof. constructor. Qed.
 
-Global Remove Hints int_elem_of_it : typeclass_instances.
-Global Existing Instance int_elem_of_it'.
-Lemma int_elem_of_it_iff z it :
-  z ∈ it ↔ int_elem_of_it z it.
-Proof.
-  rewrite /elem_of/int_elem_of_it' MinInt_eq MaxInt_eq//.
-Qed.
-Lemma ly_align_log_in_u8 ly :
-  ly_align_in_bounds ly → Z.of_nat (ly_align_log ly) ∈ u8.
-Proof.
-  apply ly_align_log_in_u8.
-Qed.
-Lemma ly_align_log_in_usize ly :
-  ly_align_in_bounds ly → Z.of_nat (ly_align_log ly) ∈ usize_t.
-Proof.
-  apply ly_align_log_in_usize.
-Qed.
-Lemma ly_align_in_usize ly :
-  ly_align_in_bounds ly → Z.of_nat (ly_align ly) ∈ usize_t.
-Proof.
-  apply ly_align_in_usize.
-Qed.
-
 (** Block typeclass resolution for an argument *)
 Definition TCNoResolve (P : Type) := P.
 Global Typeclasses Opaque TCNoResolve.
