theories/rust_typing/int.v
@@ -34,12 +34,12 @@ Section int.
   Qed.
 
   Lemma ty_own_int_in_range l π n it : l ◁ᵥ{π} n @ int it -∗ ⌜n ∈ it⌝.
-  Proof. iIntros "[%Hl _]". iPureIntro. rewrite int_elem_of_it_iff. by eapply val_to_Z_in_range. Qed.
+  Proof. iIntros "[%Hl _]". iPureIntro. by eapply val_to_Z_in_range. Qed.
 
   Lemma ty_shr_int_in_range l π κ n it : l ◁ₗ{π, κ} n @ int it -∗ ▷ ⌜n ∈ it⌝.
   Proof.
     iIntros "(%v & (%ly & Hv & (Ha & _) & Halg & Hl))" => /=. iNext. iDestruct "Ha" as "%Hn".
-    iPureIntro. apply int_elem_of_it_iff. by eapply val_to_Z_in_range.
+    iPureIntro. by eapply val_to_Z_in_range.
   Qed.
 
   Global Instance int_copyable it : Copyable (int it).
